\documentclass{homework}
\input{../homework_shared.tex}
\input{../../standardcmd.tex}


\newcommand{\hwnum}{9}
\renewcommand{\questiontype}{Problem}

\begin{document}
	\maketitle
	
	\question
	\newcommand{\atwo}{A^{(2)}}
	Let $A$ be a nonsingular matrix, and let $\atwo$ be the matrix from the lecture slides in the second step of Gaussian elimination. Then there exists $s \ge 2$ such that $a_{2s}^{(2)} \ne 0$.
	\begin{proof}
		Suppose on the contrary. By the Gaussian elimination process, we know that $a_{21}^{(2)} = 0$. If there is no $s \ge 2$ such that $a_{2s}^{(2)} \ne 0$, then the whole second row of $\atwo$ is zero. Hence, expanding by cofactors along the second row, we see that the determinant of $\atwo$ is
		\begin{equation}
			\det\left(\atwo\right) = 0\cdot\det(B_1) + 0\cdot\det(B_2) + \cdots +0\cdot\det(B_n) = 0,
		\end{equation}
		where $B_i$ is the cofactor corresponding to $a^{(2)}_{2i}$. Then $\atwo$ is singular.
		
		This is a contradiction because $\atwo$ was obtained from $A$ by elementary row operations, and $A$ was nonsingular, and applying row operations to a nonsingular matrix must result in a nonsingular matrix.
	\end{proof}
	
	\question
	Let $A = \{a_{ij}\}$, and consider the SOR iteration for solving $Ax = b$:
	\begin{equation}
		x^{(k+1)}_i = (1-\sigma)x^{(k)}_i + \frac{\sigma}{a_{ii}}\left[b_i - \sum_{j=1}^{i-1}a_{ij}x^{(k+1)}_j - \sum_{j=i}^na_{ij}x^{(k)}_j\right], \qquad i=1,2,\dots,n.
	\end{equation}
	If $L$ is the lower-triangular part of $A$ and $U$ is the upper-triangular part, and $D$ is the diagonal, so that $A = L + U +D$, then the SOR iteration becomes
	\begin{align}
		x^{(k+1)} &= (1-\sigma)x^{(k)} + \sigma D^{-1}\left[b -Lx^{(k+1)} - Ux^{(k)}\right] \\
		\implies (D + \sigma L)x^{(k+1)} &= ((1-\sigma)D-\sigma U)x^{(k)} + \sigma b \\
		\implies x^{(k+1)} &= \left(L + \frac{1}{\sigma}D\right)^{-1}\left(\frac{1}{\sigma}D - D - U\right)x^{(k)} + \left(L + \frac{1}{\sigma}D\right)^{-1}b \\
		&= -\left(L+\frac{1}{\sigma}D\right)^{-1}\left(D - \frac{1}{\sigma}D +U\right)x^{(k)} +\left(L+\frac{1}{\sigma}D\right)^{-1}b.
	\end{align}
	Define $M = L + \frac{1}{\sigma}D$, and $N = -\left(D-\frac{1}{\sigma}D+U\right)$. Then
	\begin{equation}
		x^{(k+1)} = M^{-1}Nx^{(k)} + M^{-1}b,
	\end{equation}
	and
	\begin{equation}
		A = L + D + U = \left(L+\frac{1}{\sigma}D\right) + \left(D - \frac{1}{\sigma}D + U\right) = M - N.
	\end{equation}
	Therefore, SOR is an iterative method that uses the $M$ and $N$ defined above.
	
	\question
	
\end{document}